move function body lemmas into separate files main file is verif_memmgr.v and verif_malloc.v is obsolete

memmgr/verif_memmgr.v
@@ -1,5 +1,9 @@
-(*+ SUPERSEDED BY main file verif_memmgr.v and verif_* for body lemmas *)
+(*+ specs and background for memmgr *)
 
+(* The code verifications are in separate files, e.g., 
+   verif_malloc_free.v proves the two main function bodies.
+   Although some lemmas are only used to verify a single function,
+   they're collected here to facilitate possible reorganization later. *)
 
 Require Import VST.floyd.proofauto.
 Require Import VST.floyd.library.
@@ -24,7 +28,7 @@ Ltac bdestruct X :=
        [ | try first [apply not_lt in H | apply not_le in H]]].
 
 (* A bit of infrastructure for brute force proof of claim3. 
-   TODO consider using Zseq in place of seq in mm_inv. 
+   TODO consider using Zseq in place of seq in mem_mgr. 
 *)
 Definition Zseq n := 
   if n <? 0 then [] else map Z.of_nat (seq 0 (Z.to_nat n)).
@@ -493,10 +497,10 @@ padding and is used e.g. in proof of body_free.
 that's not enough.)
 
 About waste: for small chunks, there is waste at the beginning of each big 
-block used by fill_bin, and mm_inv accounts for it. In addition, there is 
-waste of size s - n at the end of each small chunk (as n gets rounded
-up to the nearest size2binZ), and each large chunk has waste at the start,
-for alignment; these are accounted for by malloc_token.
+block used by fill_bin, and the module invariant mem_mgr accounts for it. 
+In addition, there is waste of size s - n at the end of each small chunk 
+(as n gets rounded up to the nearest size2binZ), and each large chunk has 
+waste at the start, for alignment; these are accounted for by malloc_token.
 
 About the share: The idea is that one might want to be able to split tokens,
 though there doesn't seem to be a compelling case for that.  To do so, the API
@@ -826,7 +830,7 @@ intros. generalize dependent r. induction n.
 Qed.
 
 
-(*+ module invariant mm_inv *)
+(*+ module invariant mem_mgr *)
 
 (* There is an array, its elements point to null-terminated lists 
 of right size chunks, and there is some wasted memory.
@@ -883,7 +887,7 @@ Proof.
 Qed.
 
 
-Definition mm_inv (gv: globals): mpred := 
+Definition mem_mgr (gv: globals): mpred := 
   EX bins: list val, EX lens: list nat, EX idxs: list Z,
     !! (Zlength bins = BINS /\ Zlength lens = BINS /\
         idxs = map Z.of_nat (seq 0 (Z.to_nat BINS))) &&
@@ -912,7 +916,7 @@ Proof.
   rewrite sepcon_assoc. reflexivity.
 Qed.
 
-Lemma mm_inv_split':
+Lemma mem_mgr_split':
  forall b:Z, forall bins lens idxs,
      0 <= b < BINS -> Zlength bins = BINS -> Zlength lens = BINS -> 
      idxs = map Z.of_nat (seq 0 (Z.to_nat BINS)) ->
@@ -952,9 +956,9 @@ Proof.
 Qed.
 
 
-Lemma mm_inv_split: 
+Lemma mem_mgr_split: 
  forall gv:globals, forall b:Z, 0 <= b < BINS ->
-   mm_inv gv
+   mem_mgr gv
  = 
   EX bins: list val, EX lens: list nat, EX idxs: list Z,
     !! (Zlength bins = BINS /\ Zlength lens = BINS /\ Zlength idxs = BINS 
@@ -967,13 +971,13 @@ Lemma mm_inv_split:
 Proof. 
   intros. apply pred_ext.
   - (* LHS -> RHS *)
-    unfold mm_inv.
+    unfold mem_mgr.
     Intros bins lens idxs. Exists bins lens idxs. entailer!.
-    rewrite <- (mm_inv_split' b); try assumption. 
+    rewrite <- (mem_mgr_split' b); try assumption. 
     entailer!. reflexivity.
   - (* RHS -> LHS *)
     Intros bins lens idxs. 
-    unfold mm_inv. Exists bins lens idxs. 
+    unfold mem_mgr. Exists bins lens idxs. 
     entailer!.
     set (idxs:=(map Z.of_nat (seq 0 (Z.to_nat BINS)))).
     replace (
@@ -985,7 +989,7 @@ Proof.
           iter_sepcon mmlist' (sublist (b + 1) BINS (zip3 lens bins idxs)) *
           mmlist (bin2sizeZ b) (Znth b lens) (Znth b bins) nullval )
       by (apply pred_ext; entailer!).  
-    rewrite (mm_inv_split' b); try assumption.
+    rewrite (mem_mgr_split' b); try assumption.
     cancel.  auto.
 Qed.
 
@@ -1377,7 +1381,7 @@ Qed.
 (*+ code specs *)
 
 
-(* Similar to current specs in floyd/library, with mm_inv added and size bound 
+(* Similar to current specs in floyd/library, with mem_mgr added and size bound 
 revised to account for the header of size WORD and its associated alignment.
 Also free allows null, as per Posix standard.
 
@@ -1391,11 +1395,11 @@ Definition malloc_spec {cs: compspecs } :=
              complete_legal_cosu_type t = true;
              natural_aligned natural_alignment t = true)
        LOCAL (temp _nbytes (Vptrofs (Ptrofs.repr (sizeof t))); gvars gv)
-       SEP ( mm_inv gv )
+       SEP ( mem_mgr gv )
    POST [ tptr tvoid ] EX p:_,
        PROP ()
        LOCAL (temp ret_temp p)
-       SEP ( mm_inv gv;
+       SEP ( mem_mgr gv;
              if eq_dec p nullval then emp
              else (malloc_token Tsh t p * data_at_ Tsh t p)).
 
@@ -1405,13 +1409,13 @@ Definition free_spec {cs:compspecs} :=
    PRE [ _p OF tptr tvoid ]
        PROP ()
        LOCAL (temp _p p; gvars gv)
-       SEP (mm_inv gv; 
+       SEP (mem_mgr gv; 
             if eq_dec p nullval then emp
             else (malloc_token Tsh t p * data_at_ Tsh t p))
    POST [ Tvoid ]
        PROP ()
        LOCAL ( )
-       SEP (mm_inv gv).
+       SEP (mem_mgr gv).
 
 Definition malloc_small_spec :=
    DECLARE _malloc_small
@@ -1421,17 +1425,17 @@ Definition malloc_small_spec :=
              complete_legal_cosu_type t = true /\
              natural_aligned natural_alignment t = true)
        LOCAL (temp _nbytes (Vptrofs (Ptrofs.repr (sizeof t))); gvars gv)
-       SEP ( mm_inv gv )
+       SEP ( mem_mgr gv )
    POST [ tptr tvoid ] EX p:_,
        PROP ()
        LOCAL (temp ret_temp p)
-       SEP ( mm_inv gv; 
+       SEP ( mem_mgr gv; 
             if eq_dec p nullval then emp
             else (malloc_token Tsh t p * data_at_ Tsh t p)).
 
 (* Note that this is a static function so there's no need to hide
 globals in its spec; but that seems to be needed, given the definition 
-of mm_inv.*)
+of mem_mgr.*)
 Definition malloc_large_spec :=
    DECLARE _malloc_large
    WITH t:type, gv:globals
@@ -1440,11 +1444,11 @@ Definition malloc_large_spec :=
              complete_legal_cosu_type t = true /\
              natural_aligned natural_alignment t = true)
        LOCAL (temp _nbytes (Vptrofs (Ptrofs.repr (sizeof t))); gvars gv)
-       SEP ( mm_inv gv )
+       SEP ( mem_mgr gv )
    POST [ tptr tvoid ] EX p:_,
        PROP ()
        LOCAL (temp ret_temp p)
-       SEP ( mm_inv gv; 
+       SEP ( mem_mgr gv; 
             if eq_dec p nullval then emp
             else (malloc_token Tsh t p * data_at_ Tsh t p)).
 
@@ -1460,11 +1464,11 @@ Definition free_small_spec :=
        SEP ( data_at Tsh tuint (Vptrofs (Ptrofs.repr s)) (offset_val (- WORD) p); 
             data_at_ Tsh (tptr tvoid) p;
             memory_block Tsh (s - WORD) (offset_val WORD p);
-            mm_inv gv)
+            mem_mgr gv)
    POST [ tvoid ]
        PROP ()
        LOCAL ()
-       SEP (mm_inv gv).
+       SEP (mem_mgr gv).
 
 (* The postcondition describes the list returned, together with
    TT for the wasted space at the beginning and end of the big block from mmap. *)
@@ -1487,104 +1491,6 @@ Definition Gprog : funspecs :=
    free_spec]).
 
 (*+ code correctness *)
-
-Lemma body_bin2size: semax_body Vprog Gprog f_bin2size bin2size_spec.
-Proof. start_function. forward. 
-Qed.
-
-
-Lemma body_size2bin: semax_body Vprog Gprog f_size2bin size2bin_spec.
-Proof. start_function. 
-  forward_call (BINS-1). rep_omega. 
-  forward_if.
-  - (* then *) 
-    forward. entailer!. f_equal. f_equal. unfold size2binZ; simpl. 
-    bdestruct (bin2sizeZ (BINS - 1) <? s); try omega.
-  - (* else *)
-    forward.  entailer!. f_equal. unfold size2binZ. 
-    bdestruct (bin2sizeZ (BINS - 1) <? s); try omega.
-    unfold Int.divu. do 2 rewrite Int.unsigned_repr by rep_omega. 
-    f_equal. normalize.  f_equal. rep_omega.
-Qed.
-
-
-(* Invariant for loop in fill_bin.
-p, s, N are fixed
-s + WORD is size of a (small) chunk (including header)
-         and we will have s = bin2sizeZ(b) for 0<=b<BINS
-p is start of the big block
-N is the number of chunks that fit following the waste prefix of size WA
-q points to the beginning of a list chunk (size field), unlike the link field
-which points to the link field of the following chunk.
-*)
-Definition fill_bin_inv (p:val) (s:Z) (N:Z) := 
-  EX j:_,
-  PROP ( N = (BIGBLOCK-WA) / (s+WORD) /\ 0 <= j < N /\
-         align_compatible (tarray tuint 1) (offset_val (WA+(j*(s+WORD))) p) (* q *)
-)  
-(* j remains strictly smaller than N because j is the number 
-of finished chunks and the last chunk gets finished following the loop. *)
-  LOCAL( temp _q (offset_val (WA+(j*(s+WORD))) p);
-         temp _p p; 
-         temp _s       (Vint (Int.repr s));
-         temp _Nblocks (Vint (Int.repr N));
-         temp _j       (Vint (Int.repr j)))  
-(* (offset_val (WA + ... + WORD) p) accounts for waste plus M many chunks plus
-the offset for size field.  The last chunk's nxt points one word _inside_ 
-the remaining part of the big block. *)
-  SEP (memory_block Tsh WA p; (* initial waste *)
-       mmlist s (Z.to_nat j) (offset_val (WA + WORD) p) 
-                             (offset_val (WA + (j*(s+WORD)) + WORD) p); 
-       memory_block Tsh (BIGBLOCK-(WA+j*(s+WORD))) (offset_val (WA+(j*(s+WORD))) p)). 
-
-
-Lemma fill_bin_inv_remainder':
-(* The invariant says there's a memory_block at q of size (BIGBLOCK-(WA+j*(s+WORD))),
-and later we state that q+WORD is malloc_compatible for ((N-j)*(s+WORD) - WORD).  *)
-  forall N s j,
-  N = (BIGBLOCK-WA) / (s+WORD) -> 0 <= s -> 0 <= j < N -> 
-  BIGBLOCK-(WA+j*(s+WORD)) = (N-j)*(s+WORD) + (BIGBLOCK-WA) mod (s+WORD). 
-Proof.
-  intros.
-  assert ((BIGBLOCK - WA) 
-          = (s+WORD) * ((BIGBLOCK - WA)/(s+WORD)) + (BIGBLOCK - WA) mod (s+WORD)) 
-    by (apply Z_div_mod_eq; rep_omega).
-  rewrite Z.sub_add_distr.
-  replace ((BIGBLOCK-WA) mod (s+WORD))%Z
-    with ((BIGBLOCK-WA) mod (s+WORD) + j*(s+WORD) - j*(s+WORD))%Z by omega.
-  assert (Hsub_cancel_r: forall p n m, n = m -> n-p = m-p)    (* klunky *) 
-    by (intros; eapply Z.sub_cancel_r; assumption).
-  replace 
-    ((N - j) * (s + WORD) + ((BIGBLOCK - WA) mod (s + WORD) + j * (s + WORD) - j * (s + WORD)))
-    with (((N - j) * (s + WORD) + ((BIGBLOCK - WA) mod (s + WORD) + j * (s + WORD)) - j * (s + WORD))) by omega.
-  apply Hsub_cancel_r.
-  replace ((N - j) * (s + WORD) + ((BIGBLOCK - WA) mod (s + WORD) + j * (s + WORD)))
-    with ( (N - j)*(s + WORD) + j*(s + WORD) + (BIGBLOCK - WA) mod (s + WORD) ) by omega.
-  replace ( (N - j)*(s + WORD) + j*(s + WORD) )%Z 
-    with ( N * (s + WORD) )%Z by lia.
-  replace (N*(s+WORD))%Z with ((s+WORD)*N)%Z by lia; subst N; auto.
-Qed.
-
-Lemma fill_bin_inv_remainder:
-(* consequence of fill_bin_inv and the loop guard (j<N-1) *)
-  forall N s j, N = (BIGBLOCK-WA) / (s+WORD) -> WORD <= s -> 0 <= j < N-1 -> 
-  WORD < BIGBLOCK - (WA + j * (s + WORD)) - (s + WORD).
-Proof.
-  intros N s j H H0 H1.
-  erewrite fill_bin_inv_remainder'; try apply H; try rep_omega.
-  assert (N - j >= 2) by omega.
-  assert (0 <= (BIGBLOCK - WA) mod (s + WORD)) by (apply Z_mod_lt; rep_omega).
-  assert ( (N-j)*(s+WORD) > (s+WORD) ).
-  { replace (s+WORD) with (1 * (s+WORD))%Z at 2 by omega; 
-     apply Zmult_gt_compat_r; rep_omega.
-  }
-  assert( (N - j) * (s + WORD) - (s + WORD)
-          <= (N - j) * (s + WORD) + (BIGBLOCK - WA) mod (s + WORD) - (s + WORD) ) as H5 by rep_omega.
-  eapply Z.lt_le_trans; try apply H5.
-  assert ((N - j) * (s + WORD) >= (s+WORD)+(s+WORD)) by nia.
-  assert ((N - j) * (s + WORD) - (s+WORD) >= (s+WORD)) by omega.
-  apply (Z.lt_le_trans _ (s+WORD) _); try rep_omega.
-Qed.
 
 
 Lemma malloc_compat_WORD_q:
@@ -1716,195 +1622,6 @@ Proof.
 Qed.
 
 
-Lemma body_malloc:  semax_body Vprog Gprog f_malloc malloc_spec.
-Proof. 
-start_function. 
-forward_call (BINS-1). (*! t'3 = bin2size(BINS-1) !*)
-rep_omega. 
-forward_if. (*! if nbytes > t'3 !*)
-- (* case nbytes > bin2size(BINS-1) *)
-  forward_call (t, gv).  (*! t'1 = malloc_large(nbytes) !*)
-  { (* precond *) 
-    destruct H. split3; try assumption. split; try rep_omega. 
-    assert (0 <= sizeof t) as H' by omega.
-    pose proof (unsigned_repr_le (sizeof t) H').
-    eapply Z.lt_le_trans. 
-    match goal with | HA: bin2sizeZ (BINS-1) < _ |- _ => apply HA end. 
-    assumption.
-  } 
-  Intros p.
-  forward. (*! return t'1 !*) 
-  if_tac.
-  + (* case p = null *) Exists nullval. entailer!.
-    if_tac; try contradiction. entailer!. 
-  + Exists p. if_tac. contradiction. 
-    entailer!.  
-- (* case nbytes <= bin2size(BINS-1) *)
-  forward_call(t,gv).  (*! t'2 = malloc_small(nbytes) !*)
-  { (* precond *)
-    destruct H. split3; try assumption. 
-    split; try rep_omega. 
-    clear H0 H1.
-    match goal with | HA: bin2sizeZ (BINS-1) >= _ |- _ => apply Z.ge_le in HA end.
-    rewrite max_unsigned_32 in *.
-    rewrite Int.unsigned_repr in *; try assumption. 
-    split; try omega. 
-    apply Z.lt_le_incl; assumption.
-    assert (0 <= WA+WORD) as HA by rep_omega.
-    eapply Z.le_le_sub_lt; try apply HA.
-    replace (sizeof t - 0) with (sizeof t).
-    assumption.
-    rewrite Z.sub_0_r; reflexivity.
-  }
-  Intros p.
-  forward. (*! result = t'2 !*)
-  Exists p. 
-  entailer!.
-Qed.
-
-Lemma body_free:  semax_body Vprog Gprog f_free free_spec.
-Proof. 
-start_function. 
-set (n:=sizeof t). (* try to avoid entailer or rep_omega issues *)
-forward_if (PROP()LOCAL()SEP(mm_inv gv)). (*! if (p != NULL) !*)
-- (* typecheck *) if_tac. entailer!.
-  assert_PROP( 0 < n ) by (unfold malloc_token; unfold malloc_tok; entailer).
-  sep_apply (data_at__memory_block Tsh t p). 
-  entailer!.
-- (* case p!=NULL *)
-  apply semax_pre with 
-   (PROP ( )
-     LOCAL (temp _p p; gvars gv)
-     SEP (mm_inv gv;  malloc_token Tsh t p * data_at_ Tsh t p)).
-  { if_tac; entailer!. }
-  assert_PROP ( 0 <= n <= Ptrofs.max_unsigned - WORD ) by entailer!. 
-  sep_apply (from_malloc_token_and_block t n p); auto.
-  Intros s.
-  assert_PROP( 
-     (force_val
-     (sem_add_ptr_int tuint Signed (force_val (sem_cast_pointer p))
-        (eval_unop Oneg tint (Vint (Int.repr 1)))) 
-    = field_address tuint [] (offset_val (- WORD) p))).
-  { entailer!. simpl. unfold field_address. if_tac. normalize. contradiction. }
-  forward. (*! t'2 = p[-1] !*)
-  forward. (*! s = t'2 !*) 
-  forward_call(BINS - 1). (*! t'1 = bin2size(BINS - 1) !*)
-  { (* precond *) rep_omega. } 
-  deadvars!.
-  forward_if (PROP () LOCAL () SEP (mm_inv gv)). (*! if s <= t'1 !*)
-  -- (* case s <= bin2sizeZ(BINS-1) *)
-    forward_call(p,s,n,gv). (*! free_small(p,s) !*) 
-    { (* preconds *) split3; try omega; try assumption. }
-    entailer!. if_tac. entailer. omega.
-  -- (* case s > bin2sizeZ(BINS-1) *)
-    if_tac; try omega.
-    (*! munmap( p-(WASTE+WORD), s+WASTE+WORD ) !*)
-    forward_call( (offset_val (-(WA+WORD)) p), (s+WA+WORD) ).
-    + entailer!. destruct p; try contradiction; simpl. normalize.
-      rewrite Ptrofs.sub_add_opp. reflexivity.
-    + (* munmap pre *)
-      entailer!. 
-      sep_apply (free_large_chunk s p); try rep_omega.
-      entailer!.
-    + rep_omega.
-    + entailer!.
-- (* case p == NULL *) 
-  forward. (*! skip !*)
-  entailer!.
-- (* after if *)
-  forward. (*! return !*)
-Qed.
-
-Lemma body_malloc_large: semax_body Vprog Gprog f_malloc_large malloc_large_spec.
-Proof.
-start_function. 
-set (n:= sizeof t).
-forward_call (n+WA+WORD). (*! t'1 = mmap0(nbytes+WASTE+WORD ...) !*)
-{ rep_omega. }
-Intros p.
-(* NOTE could split cases here; then two symbolic executions but simpler ones *)
-forward_if. (*! if (p==NULL) !*)
-- (* typecheck guard *) 
-  if_tac; entailer!.
-- (* case p == NULL *) 
-  forward. (*! return NULL  !*)
-  Exists (Vint (Int.repr 0)).
-  if_tac; entailer!. (* cases in post of mmap *)
-- (* case p <> NULL *) 
-  if_tac. (* cases in post of mmap *)
-  + (* impossible case *)
-    elimtype False. destruct p; try contradiction; simpl in *.
-  + assert_PROP (
-        (force_val
-           (sem_add_ptr_int tuint Signed
-                            (force_val
-                               (sem_cast_pointer
-                                  (force_val
-                                     (sem_add_ptr_int tschar Unsigned p
-                                                      (Vint
-                                                         (Int.sub
-                                                            (Int.mul (Ptrofs.to_int (Ptrofs.repr 4)) (Int.repr 2))
-                                                            (Ptrofs.to_int (Ptrofs.repr 4))))))))
-                            (Vint (Int.repr 0))) = field_address tuint [] (offset_val WA p)) ).
-    (* painful pointer reasoning to enable forward (p+WASTE)[0] = nbytes *)
-    { entailer!. 
-      destruct p; try contradiction; simpl.
-      normalize.
-      unfold field_address.
-      rewrite if_true.
-      { simpl.  normalize. }
-      hnf. (* drill down *) 
-      repeat split; auto.
-      - (* size compat *)
-        red. 
-        match goal with | H:size_compatible' _ _ |- _ => red in H end.
-        unfold Ptrofs.add.
-        rewrite (Ptrofs.unsigned_repr WA) by rep_omega.
-        rewrite Ptrofs.unsigned_repr by rep_omega.
-        simpl sizeof. rep_omega.
-      - (* align compat *)
-        red.
-        eapply align_compatible_rec_by_value; try reflexivity.
-        simpl in *. unfold natural_alignment in *. unfold Z.divide in *.
-        match goal with | HA: (exists z:Z, _) /\ _ |- _ => destruct HA as [Hz Hlim] end. 
-        inv Hz.
-        rewrite <- (Ptrofs.repr_unsigned i). 
-        match goal with | HA: Ptrofs.unsigned _ = _ |- _ => rewrite HA end. 
-        exists (2*x+1). change WA with 4.
-        rewrite ptrofs_add_repr. rewrite Ptrofs.unsigned_repr.
-        omega. rep_omega.
-    }
-    rewrite malloc_large_chunk; try rep_omega; try assumption.
-    Intros. (* flatten sep *)
-    forward. (*! (p+WASTE)[0] = nbytes;  !*)
-    forward. (*! return (p+WASTE+WORD);  !*)
-    (* postcond *)
-    Exists (offset_val (WA+WORD) p).
-    entailer!.  
-    if_tac. 
-    { elimtype False. destruct p; try contradiction; simpl in *. 
-      match goal with | HA: Vptr _ _  = nullval |- _ => inv HA end. }
-    entailer!.
-    unfold malloc_token.
-    Exists n.
-    unfold malloc_tok.
-    if_tac. rep_omega. entailer!. 
-    { apply malloc_compatible_offset; try rep_omega; try apply WORD_ALIGN_aligned.
-      replace (n+(WA+WORD)) with (n + WA + WORD) by omega. assumption. }
-    cancel.
-    (* data_at_ from memory_block *)
-    replace (n - sizeof t) with 0 by omega.
-    rewrite memory_block_zero.  entailer!.
-    subst n.
-    rewrite memory_block_data_at_. entailer!.
-    destruct H as [Hsz [Hcosu Halign]]; auto.
-    apply malloc_compatible_field_compatible; try auto.
-    apply malloc_compatible_offset; try rep_omega.
-    replace (sizeof t + (WA + WORD)) with (sizeof t + WA + WORD) by omega; assumption.
-    apply WORD_ALIGN_aligned.
-Qed.
-
-
 Lemma Zdiv_prod:
   forall a b c, (a*b|c) -> (a|c).
 Proof.
@@ -1929,618 +1646,8 @@ Proof.
 Qed.
 
 
-Lemma body_fill_bin: semax_body Vprog Gprog f_fill_bin fill_bin_spec.
-Proof. 
-start_function. 
-forward_call b.  (*! s = bin2size(b) !*)
-set (s:=bin2sizeZ b).
-assert (WORD <= s <= bin2sizeZ(BINS-1)) by (pose proof (bin2size_range b); rep_omega).
-forward_call BIGBLOCK.  (*! *p = mmap0(BIGBLOCK ...) !*)  
-{ rep_omega. }
-Intros p.
-if_tac in H1. (* split cases on mmap post *)
-- (* case p = nullval *)
-  forward_if. (*! if p == NULL !*)
-  (* case p <> nullval *)
-  forward. (*! return NULL !*)
-  Exists nullval. Exists 1. 
-  entailer!.  if_tac; try contradiction. entailer!. contradiction.
-- (* case p <> nullval *)
-  assert_PROP (isptr p) by entailer!.
-  destruct p; try contradiction. 
-  rename b0 into pblk; rename i into poff. (* p as blk+ofs *)
-  assert_PROP (Ptrofs.unsigned poff + BIGBLOCK < Ptrofs.modulus) by entailer!.
-  forward_if; try contradiction.
-  match goal with | HA: ?a = ?a |- _  => clear HA end.
-  forward. (*! Nblocks = (BIGBLOCK-WASTE) / (s+WORD) !*)
-  { (* nonzero divisor *) entailer!.
-    match goal with 
-    | HA: Int.repr _ = _  |- _  
-      => apply repr_inj_unsigned in HA; rep_omega end. }
-  deadvars!. 
-  forward. (*! q = p + WASTE !*)
-  forward. (*! j = 0 !*) 
-  forward_while (*! while (j != Nblocks - 1) !*) 
-    (fill_bin_inv (Vptr pblk poff) s ((BIGBLOCK-WA) / (s+WORD)) ).
-* (* pre implies inv *)
-  Exists 0. 
-  entailer!.
-  ** repeat (try split; try rep_omega).
-     *** apply BIGBLOCK_enough; rep_omega. 
-     *** (* TODO alignment of q -- once all proved, make a tactic for this mess *)
-       eapply align_compatible_rec_Tarray; try reflexivity.
-       intros. assert (Hi: i=0) by omega; subst i; simpl; clear H6.
-       match goal with | |- context[(Ptrofs.unsigned ?e + 0)] =>
-         replace (Ptrofs.unsigned e + 0) with (Ptrofs.unsigned e) by omega end.
-       eapply align_compatible_rec_by_value; try reflexivity.
-       unfold align_chunk.
-       assert (Hpoff: (8 | Ptrofs.unsigned poff)) 
-         by (unfold malloc_compatible in H1; destruct H1 as [Halign Hsize]; auto).
-       rewrite Mem.addressing_int64_split; auto.
-       apply Z.divide_add_r; auto.
-       replace 8 with (4*2)%Z in Hpoff by omega.
-       apply (Zdiv_prod _ 2 _); auto.  apply Z.divide_reflexive.
-     *** unfold Int.divu; normalize. 
-  ** replace BIGBLOCK with (WA + (BIGBLOCK - WA)) at 1 by rep_omega.
-     rewrite memory_block_split_repr; try rep_omega. entailer!.
-* (* pre implies guard defined *)
-  entailer!.
-  pose proof BIGBLOCK_enough as HB. 
-  assert (H0x: 0 <= s <= bin2sizeZ(BINS-1)) by rep_omega.
-  specialize (HB s H0x); clear H0x.
-  change (Int.signed (Int.repr 1)) with 1.
-  rewrite Int.signed_repr; rep_omega.
-* (* body preserves inv *)
-  match goal with | HA: _ /\ _ /\ _ |- _ => destruct HA as [? [? Hmc]] end.
-  match goal with | HA: ?a = ?a |- _  => clear HA end.
-  freeze [0] Fwaste. 
-  match goal with | HA: _ |- 
-        context[memory_block _ ?mm ?qq] =>set (m:=mm); set (q:=qq) end.
-  replace_in_pre
-   (memory_block Tsh m q)
-   (data_at_ Tsh (tarray tuint 1) q *
-    data_at_ Tsh (tptr tvoid) (offset_val WORD q) *
-    memory_block Tsh (s - WORD) (offset_val (WORD + WORD) q) *
-    memory_block Tsh (m - (s + WORD)) (offset_val (s + WORD) q)).
-  { set (N:=(BIGBLOCK-WA)/(s+WORD)).
-    sep_apply (memory_block_split_block s m q); 
-       try rep_omega; try entailer!; normalize; subst m.
-    ** replace (BIGBLOCK - (WA + j * (s + WORD)))
-         with (BIGBLOCK - WA - j * (s + WORD)) by omega.
-       apply BIGBLOCK_enough_j; rep_omega.
-    ** apply (malloc_compat_WORD_q N j (Vptr pblk poff)); auto; try rep_omega.
-       subst s; apply bin2size_align; auto.
-  }
-  Intros. (* flattens the SEP clause *) 
-  forward. (*! q[0] = s; !*) 
-  freeze [1; 2; 4; 5] fr1.  
-  forward. (*! *(q+WORD) = q+WORD+(s+WORD); !*)
-  forward. (*! q += s+WORD; !*)
-  forward. (*! j++; !*) 
-  { (* typecheck *) 
-    entailer!.
-    pose proof BIGBLOCK_enough. 
-    assert (H0x: 0 <= s <= bin2sizeZ(BINS-1)) by rep_omega.
-    match goal with | HA: forall _ : _, _ |- _ =>
-                specialize (HA s H0x) as Hrng; clear H0x end. 
-    assert (Hx: Int.min_signed <= j+1) by rep_omega.
-    split. rewrite Int.signed_repr. rewrite Int.signed_repr. assumption.
-    rep_omega. rep_omega. rewrite Int.signed_repr. rewrite Int.signed_repr.
-    assert (Hxx: j + 1 <= (BIGBLOCK-WA)/(s+WORD)) by omega.
-    apply (Z.le_trans (j+1) ((BIGBLOCK-WA)/(s+WORD))).
-    assumption. rep_omega. rep_omega. rep_omega. 
-  } 
-  (* reestablish inv *)  
-  Exists (j+1).  
-  assert (Hdist: ((j+1)*(s+WORD))%Z = j*(s+WORD) + (s+WORD))
-    by (rewrite Z.mul_add_distr_r; omega). 
-  entailer!. 
-  ** (* pure *)
-     assert (HRE' : j <> ((BIGBLOCK - WA) / (s + WORD) - 1)) 
-       by (apply repr_neq_e; assumption). 
-     assert (HRE2: j+1 < (BIGBLOCK-WA)/(s+WORD)) by rep_omega.  
-     split. 
-     *** (* alignment of updated q -- TODO, tactic, also for its initial alignment above *)
-       split; try rep_omega.
-       eapply align_compatible_rec_Tarray; try reflexivity.
-       intros. assert (Hi: i=0) by omega; subst i; simpl. 
-       match goal with | |- context[(Ptrofs.unsigned ?e + 0)] =>
-         replace (Ptrofs.unsigned e + 0) with (Ptrofs.unsigned e) by omega end.
-       eapply align_compatible_rec_by_value; try reflexivity.
-       unfold align_chunk.
-       assert (Hpoff: (8 | Ptrofs.unsigned poff)) 
-         by (unfold malloc_compatible in H1; destruct H1 as [Halign Hsize]; auto).
-       assert (Hpoff': (4 | Ptrofs.unsigned poff)) by 
-           (replace 8 with (4*2)%Z in Hpoff by omega; apply (Zdiv_prod _ 2 _); auto).  
-       assert (HWA: (4 | WA)) by (rewrite WA_eq; apply Z.divide_reflexive).
-       assert (Hrest: (natural_alignment | (j+1)*(s+WORD)))
-         by (apply Z.divide_mul_r; subst s; apply bin2size_align; auto).
-       unfold natural_alignment in Hrest.
-       assert (Hrest' : (4 | (j + 1) * (s + WORD)))
-         by (replace 8 with (4*2)%Z in Hrest by omega; apply (Zdiv_prod _ 2 _); auto).  
-       clear Hpoff Hrest H7 H8.
-       assert (Hz: (4 | WA + (j + 1) * (s + WORD))) by (apply Z.divide_add_r; auto).
-       clear HWA Hpoff' Hrest'.
-       rewrite ptrofs_add_for_alignment.
-       **** apply Z.divide_add_r; try assumption.
-            match goal with | HA: malloc_compatible _ _ |- _ => 
-                              simpl in HA; destruct HA as [Hal Hsz] end.
-            assert (H48: (4|natural_alignment)).
-            { unfold natural_alignment; replace 8 with (2*4)%Z by omega. 
-              apply Z.divide_factor_r; auto. }
-            eapply Z.divide_trans. apply H48. auto.
-       **** assert (j+1>0) by omega; assert (s+WORD>0) by rep_omega.
-            assert ((j+1)*(s+WORD) > 0) by (apply Zmult_gt_0_compat; auto).
-            rep_omega.
-       **** match goal with | HA: malloc_compatible _ _ |- _ => 
-                              simpl in HA; destruct HA as [Hal Hsz] end.
-            change Ptrofs.max_unsigned with (Ptrofs.modulus - 1).
-            (* aiming to use Hsz *)
-            assert (WA + (j + 1) * (s + WORD) <= BIGBLOCK).
-            { assert (H0s: 0 <= s) by rep_omega.
-              pose proof (BIGBLOCK_enough_j s (j+1) H0s HRE2);  rep_omega. 
-            }
-            rep_omega.
-     *** assert (H': 
-               BIGBLOCK - WA - ((BIGBLOCK-WA)/(s+WORD)) * (s + WORD) 
-               < BIGBLOCK - WA - (j + 1) * (s + WORD))
-       by (apply Z.sub_lt_mono_l; apply Z.mul_lt_mono_pos_r; rep_omega).
-         do 3 f_equal; rep_omega.
-  ** (* spatial *)
-     thaw fr1. thaw Fwaste; cancel. (* thaw and cancel the waste *)
-    (* aiming to fold list by lemma mmlist_fold_last, first rewrite conjuncts *)
-    set (r:=(offset_val (WA + WORD) (Vptr pblk poff))). (* r is start of list *)
-    replace (offset_val (WA + j * (s + WORD) + WORD) (Vptr pblk poff)) 
-      with (offset_val WORD q) by (unfold q; normalize).
-    replace (upd_Znth 0 (default_val (tarray tuint 1) ) (Vint (Int.repr s)))
-      with [(Vint (Int.repr s))] by (unfold default_val; normalize).
-    change 4 with WORD in *. (* ugh *)
-    assert (HnxtContents: 
-    (Vptr pblk
-       (Ptrofs.add poff
-          (Ptrofs.repr (WA + j * (s + WORD) + (WORD + (s + WORD))))))
-    = (offset_val (s + WORD + WORD) q))
-      by ( simpl; f_equal; rewrite Ptrofs.add_assoc; f_equal; normalize; f_equal; omega). 
-    rewrite HnxtContents; clear HnxtContents.
-    replace (Vptr pblk (Ptrofs.add poff (Ptrofs.repr (WA + j*(s+WORD) + WORD))))
-      with  (offset_val WORD q) by (unfold q; normalize). 
-    replace (offset_val (WA + j * (s + WORD) + (WORD + WORD)) (Vptr pblk poff))
-      with  (offset_val (WORD+WORD) q ) by (unfold q; normalize). 
-    set (n:=Z.to_nat j).
-    replace (Z.to_nat (j+1)) with (n+1)%nat by 
-        (unfold n; change 1%nat with (Z.to_nat 1); rewrite Z2Nat.inj_add; auto; omega). 
-    set (m':= m - (s+WORD)).
-    assert (H0s: 0 <= s) by rep_omega.
-    pose proof (BIGBLOCK_enough_j s j H0s (proj2 H6)) as Hsw; clear H0s.
-    assert (Hmcq: malloc_compatible s (offset_val WORD  q)).
-    { assert (HmcqB:
-                malloc_compatible (BIGBLOCK - (WA + j*(s+WORD)) - WORD) (offset_val WORD q)).
-      { remember ((BIGBLOCK-WA)/(s+WORD)) as N. 
-        apply (malloc_compat_WORD_q N _ (Vptr pblk poff)); try auto.
-        rep_omega.
-        apply bin2size_align; auto.
-      }
-      apply (malloc_compatible_prefix s (BIGBLOCK-(WA+j*(s+WORD))-WORD)); try rep_omega; auto.
-    }
-    assert (Hmpos: WORD < m'). (* space remains, so we can apply mmlist_fold_last *)
-    { subst m'; subst m.
-      remember ((BIGBLOCK-WA)/(s+WORD)) as N.
-      assert (Hsp: 0 <= s) by rep_omega.
-      assert (HRE' : j <> ((BIGBLOCK - WA) / (s + WORD) - 1)) 
-        by (subst N; apply repr_neq_e; assumption).
-      assert (HjN: 0<=j<N-1) by omega; clear HRE HRE'.
-      apply (fill_bin_inv_remainder ((BIGBLOCK-WA)/(s+WORD))); rep_omega.
-    }
-    sep_apply (mmlist_fold_last s n r q m' Hmcq Hmpos); try rep_omega.
-    { subst m'. subst m.
-      replace (BIGBLOCK - (WA + j * (s + WORD)) - (s + WORD) - WORD)
-        with (BIGBLOCK - WA - j * (s + WORD) - s - WORD - WORD) by omega.
-      assert (0 <= j*(s+WORD)) by
-        (destruct H6; assert (0<=s+WORD) by rep_omega; apply Z.mul_nonneg_nonneg; rep_omega).
-      rep_omega.
-    }
-    entailer!.
-    assert (H': 
-        (Vptr pblk (Ptrofs.add poff (Ptrofs.repr (WA + (j+1)*(s+WORD) + WORD))))
-      = (offset_val (s+WORD+WORD) (offset_val (WA + j*(s+WORD)) (Vptr pblk poff)))).
-    { simpl. f_equal. rewrite Ptrofs.add_assoc. f_equal. normalize.
-      rewrite Hdist. f_equal. rep_omega. }
-    rewrite H'; clear H'.
-    unfold r; unfold m'; unfold m.
-    assert (H': (offset_val (WA + WORD) (Vptr pblk poff))
-             = (Vptr pblk (Ptrofs.add poff (Ptrofs.repr (WA + WORD)))) ) by normalize.
-    rewrite <- H'; clear H'.
-    unfold q.
-    entailer!.    
-    assert (H': (BIGBLOCK - (WA + j * (s + WORD)) - (s + WORD))
-                   = (BIGBLOCK - (WA + (j + 1) * (s + WORD))) ) by lia.
-    rewrite H'; clear H'.
-    assert (H': 
-              (offset_val (WA + j * (s + WORD) + (s + WORD)) (Vptr pblk poff))
-              = (Vptr pblk (Ptrofs.add poff (Ptrofs.repr (WA + (j + 1) * (s + WORD))))) )
-     by (replace (WA + j * (s + WORD) + (s + WORD)) with (WA + (j + 1) * (s + WORD)) by lia;
-         normalize).
-    rewrite H'; clear H'.
-    entailer!.
-* (* after the loop *) 
-(* TODO eventually: here we're setting up the assignments 
-to finish the last chunk; this is like setting up in the loop body.
-Then we fold into the list, like at the end of the loop body. 
-It would be nice to factor commonalities. *)
-
-  set (q:= (offset_val (WA + j * (s + WORD)) (Vptr pblk poff))).
-  set (m:= (BIGBLOCK - (WA + j * (s + WORD)))).
-  replace_in_pre
-   (memory_block Tsh m q)
-   (data_at_ Tsh (tarray tuint 1) q *
-    data_at_ Tsh (tptr tvoid) (offset_val WORD q) *
-    memory_block Tsh (s - WORD) (offset_val (WORD + WORD) q) *
-    memory_block Tsh (m - (s + WORD)) (offset_val (s + WORD) q)).
-  { 
-    sep_apply (memory_block_split_block s m q); try rep_omega.
-    ** subst m. replace (BIGBLOCK - (WA + j * (s + WORD)))
-              with (BIGBLOCK - WA - j * (s + WORD)) by omega.
-       apply BIGBLOCK_enough_j; rep_omega.
-    ** subst m. 
-       set (N:=(BIGBLOCK-WA)/(s+WORD)).
-       apply (malloc_compat_WORD_q N j (Vptr pblk poff)); auto; try rep_omega.
-       subst s; apply bin2size_align; auto.
-    ** destruct H5 as [H5a [H5j H5align]]; normalize.
-    ** entailer!.  
-  }
-  Intros. (* flattens the SEP clause *) 
-  freeze [0;5] Fwaste. (* discard what's not needed for post *)
-  forward. (*! q[0] = s !*)
-  replace (upd_Znth 0 (default_val (tarray tuint 1) ) (Vint (Int.repr s)))
-    with [(Vint (Int.repr s))] by (unfold default_val; normalize).
-  forward. (*!  *(q+WORD) = NULL !*)
-  set (r:=(offset_val (WA + WORD) (Vptr pblk poff))).   
-  set (n:=Z.to_nat j).
-  replace (offset_val (WA + j * (s + WORD) + WORD) (Vptr pblk poff)) 
-    with (offset_val WORD q) by (subst q; normalize).
-  assert (Hmc: malloc_compatible s (offset_val WORD q)).
-  { (* malloc_compat, for mmlist_fold_last_null *)
-    subst q.
-    rewrite offset_offset_val.
-    replace (WA + j*(s+WORD) + WORD) with (ALIGN*WORD + j*(s+WORD)) by rep_omega.
-    apply malloc_compatible_offset; try rep_omega.
-    { (* TODO factor out repeated steps in following few *)
-      apply Z.add_nonneg_nonneg; try rep_omega.
-      assert (0<=s+WORD) by rep_omega; apply Z.mul_nonneg_nonneg; rep_omega.
-    }
-    { apply (malloc_compatible_prefix _ BIGBLOCK).
-      split.
-      apply Z.add_nonneg_nonneg; try rep_omega.
-      apply Z.add_nonneg_nonneg; try rep_omega.
-      assert (0<=s+WORD) by rep_omega; apply Z.mul_nonneg_nonneg; rep_omega.
-      destruct H5 as [H5a [[H5jlo H5jhi] H5align]]; normalize.
-      assert (Hs0: 0<=s) by rep_omega; pose proof (BIGBLOCK_enough_j s j Hs0 H5jhi).
-      rep_omega.      
-      assumption.
-    } 
-    apply Z.divide_add_r.
-    apply WORD_ALIGN_aligned.
-    apply Z.divide_mul_r.
-    apply bin2size_align; auto.
-  }
-  change (Vint(Int.repr 0)) with nullval.
-  sep_apply (mmlist_fold_last_null s n r q Hmc).
-  forward. (*! return p+WASTE+WORD !*)
-  subst n. 
-  Exists r.  Exists (j+1).
-  entailer!. 
-  if_tac; auto. rep_omega.
-  if_tac. 
-  *** (* contradiction *)
-    match goal with | HA: r = nullval <-> _, HB: r = nullval |- _ 
-                      => apply HA in HB; rep_omega end.
-  *** entailer!. subst s. 
-      replace (Z.to_nat j + 1)%nat with (Z.to_nat (j + 1))%nat.
-      entailer!.
-      rewrite Z2Nat.inj_add; try rep_omega; reflexivity.
-Qed.
-
-Lemma body_malloc_small:  semax_body Vprog Gprog f_malloc_small malloc_small_spec.
-Proof. 
-start_function. 
-set (n := sizeof t).
-rewrite <- seq_assoc.  
-forward_call n. (*! t'1 = size2bin(nbytes) !*)
-{ assert (bin2sizeZ(BINS-1) <= Ptrofs.max_unsigned) by rep_omega. rep_omega. }
-forward. (*! b = t'1 !*)
-set (b:=size2binZ n).
-assert (Hb: 0 <= b < BINS) by (apply (claim2 n); omega). 
-rewrite (mm_inv_split gv b) by apply Hb.
-Intros bins lens idxs.
-freeze [1; 3] Otherlists.
-deadvars!.
-forward. (*! p = bin[b] !*)
-forward_if(
-    EX p:val, EX len:Z,
-     PROP(p <> nullval)
-     LOCAL(temp _p p; temp _b (Vint (Int.repr b)); gvars gv)
-     SEP(FRZL Otherlists; TT; 
-         data_at Tsh (tarray (tptr tvoid) BINS) (upd_Znth b bins p) (gv _bin);
-         mmlist (bin2sizeZ b) (Z.to_nat len) p nullval)). 
-
-  + (* typecheck guard *)
-    destruct (Znth b lens). 
-    match goal with | HA: Znth b bins = nullval <-> _ |- _ => set (Hbn:=HA) end. 
-    (*Set Printing Implicit. -- to see the need for following step. *)
-    change Inhabitant_val with Vundef in Hbn.
-    ++ assert (Znth b bins = nullval) by apply (proj2 Hbn (eq_refl _)).
-       change (@Znth val Vundef) with (@Znth val Inhabitant_val).
-       replace (Znth b bins) with nullval by assumption.
-       auto with valid_pointer.
-    ++ match goal with | HA: Znth b bins = nullval <-> _ |- _ => destruct HA end.
-       assert (Znth b bins <> nullval) by
-           (assert (S n0 <> 0%nat) by congruence; auto).
-       change (Vint Int.zero) with nullval.
-       auto with valid_pointer.
-       apply denote_tc_test_eq_split; auto with valid_pointer.
-       sep_apply (mmlist_ne_valid_pointer (bin2sizeZ b) (S n0) (Znth b bins) nullval).
-       omega. change Inhabitant_val with Vundef; entailer!.
-  + (* case p==NULL *) 
-    change Inhabitant_val with Vundef in *.
-    replace (Znth b bins) with nullval by assumption.
-    assert_PROP(Znth b lens = 0%nat) as Hlen0.
-    { entailer!.
-      match goal with | HA: nullval = nullval <-> _ |- _ => (apply HA; reflexivity) end.
-    } 
-    rewrite Hlen0.
-    rewrite mmlist_empty.
-    forward_call b. (*! p = fill_bin(b) !*) 
-    Intro r_with_l; destruct r_with_l as [root len]; simpl.
-    forward_if. (*! if p==NULL !*)
-    { apply denote_tc_test_eq_split; auto with valid_pointer.
-      if_tac. entailer!.
-      sep_apply (mmlist_ne_valid_pointer (bin2sizeZ b) (Z.to_nat len) root nullval).
-      change (Z.to_nat len > 0)%nat with (0 < Z.to_nat len)%nat.
-      change 0%nat with (Z.to_nat 0). apply Z2Nat.inj_lt; rep_omega.
-      entailer!.
-    }
-    ++ (* case p==NULL after fill_bin() *) 
-      forward.
-      Exists nullval. entailer!. 
-      thaw Otherlists.
-      set (idxs:= (map Z.of_nat (seq 0 (Z.to_nat BINS)))).
-      replace (data_at Tsh (tarray (tptr tvoid) BINS) bins (gv _bin))
-         with (data_at Tsh (tarray (tptr tvoid) BINS) bins (gv _bin) * emp) 
-         by normalize.
-      rewrite <- (mmlist_empty (bin2sizeZ b)) at 2.
-      rewrite <- Hlen0 at 1.
-      unfold mm_inv. Exists bins. Exists lens. Exists idxs.
-      entailer!. 
-      match goal with | HA: (Znth b bins = _) |- _ => rewrite <- HA at 1 end.
-      rewrite (mm_inv_split' b); auto.  
-      pose proof (bin2size_range b); rep_omega.
-    ++ (* case p<>NULL *)
-      if_tac. contradiction.
-      gather_SEP 0 1. 
-      Intros.
-      forward. (*! bin[b] = p !*)
-      Exists root. Exists len.  
-      entailer. cancel. 
-    ++ pose proof (bin2size_range b); rep_omega.
-  + (* else branch p!=NULL *)
-    forward. (*! skip !*)
-    Exists (Znth b bins).  
-    Exists (Z.of_nat (nth (Z.to_nat b) lens 0%nat)). (* annoying conversion *)
-    rewrite Nat2Z.id.  
-    match goal with | HA: Zlength bins = _ |- _ => 
-                      rewrite upd_Znth_same_val by (rewrite HA; assumption) end. 
-    entailer!.
-    match goal with | HA: Zlength lens = _ |- _ => 
-                      rewrite <- nth_Znth by (rewrite HA; assumption) end.  
-    entailer.
-  + (* after if: unroll and pop mmlist *)
-    Intros p len.
-    set (s:=bin2sizeZ b).  
-    assert_PROP (len > 0).
-    { entailer. sep_apply (mmlist_ne_len s len p nullval); auto.
-      rewrite prop_sepcon. entailer!.  }
-    assert_PROP (isptr p).
-    { entailer!. unfold nullval in *.
-      match goal with | HA: p <> _ |- _ => simpl in HA end. (* not Archi.ptr64 *)
-      unfold is_pointer_or_null in *. simpl in *.
-      destruct p; try contradiction; simpl.
-      subst. contradiction. auto. }
-    rewrite (mmlist_unroll_nonempty s (Z.to_nat len) p);
-       try (rewrite Z2Nat.id; rep_omega); try assumption.
-    Intros q.
-    assert_PROP(force_val (sem_cast_pointer p) = field_address (tptr tvoid) [] p).
-    { entailer!. unfold field_address. if_tac. normalize. contradiction. }
-    forward. (*! q = *p !*)
-    forward. (*! bin[b]=q !*)
-    (* prepare token+chunk to return *)
-    deadvars!.
-    thaw Otherlists.  gather_SEP 4 5 6.
-    replace_SEP 0 (malloc_token Tsh t p * memory_block Tsh n p). 
-    go_lower.  change (-4) with (-WORD). (* ugh *)
-    apply (to_malloc_token_and_block n p q s); try assumption. 
-    destruct H as [? [? ?]].
-    unfold n; auto.
-    unfold s; unfold b; reflexivity. 
-    (* refold invariant *)
-    rewrite upd_Znth_twice by (rewrite H0; apply Hb).
-    gather_SEP 4 1 5.
-    set (lens':=(upd_Znth b lens (Nat.pred (Z.to_nat len)))).
-    set (bins':=(upd_Znth b bins (force_val (sem_cast_pointer q)))).
-    assert (Hlens: Nat.pred (Z.to_nat len) = (Znth b lens')).
-    { unfold lens'. rewrite upd_Znth_same. reflexivity. 
-      match goal with | HA: Zlength lens = _ |- _ => rewrite HA end. 
-      assumption. }
-    rewrite Hlens; clear Hlens.
-    change s with (bin2sizeZ b).
-    forward. (*! return p !*)
-    Exists p. entailer!. if_tac. contradiction. cancel.
-    unfold mm_inv. Exists bins'. Exists lens'. 
-    set (idxs:= (map Z.of_nat (seq 0 (Z.to_nat BINS)))).
-    Exists idxs. cancel.
-    subst n.
-    rewrite memory_block_data_at_.
-    entailer!.
-    match goal with | HA: Zlength lens = _ |- _ => 
-                      subst lens'; rewrite upd_Znth_Zlength; rewrite HA; auto end.
-    (* fold mm_inv *)
-    assert (Hbins': sublist 0 b bins' = sublist 0 b bins) by
-      (unfold bins'; rewrite sublist_upd_Znth_l; try reflexivity; try rep_omega).
-    assert (Hlens': sublist 0 b lens' = sublist 0 b lens) by 
-      (unfold lens'; rewrite sublist_upd_Znth_l; try reflexivity; try rep_omega).
-    assert (Hbins'': sublist (b+1) BINS bins' = sublist (b+1) BINS bins) by
-      (unfold bins'; rewrite sublist_upd_Znth_r; try reflexivity; try rep_omega).
-    assert (Hlens'': sublist (b+1) BINS lens' = sublist (b+1) BINS lens) by
-      (unfold lens'; rewrite sublist_upd_Znth_r; try reflexivity; try rep_omega).
-    assert (Hsub:  sublist 0 b (zip3 lens bins idxs)
-                 = sublist 0 b (zip3 lens' bins' idxs)).
-    { repeat rewrite sublist_zip3; try rep_omega.
-      - rewrite Hbins'. rewrite Hlens'.  reflexivity.
-      - unfold lens'; rewrite upd_Znth_Zlength; repeat rep_omega.
-      - unfold lens'; unfold bins'; rewrite upd_Znth_Zlength.
-        rewrite upd_Znth_Zlength; rep_omega. rep_omega.
-      - replace (Zlength bins') with BINS by auto. unfold idxs; auto.
-      - unfold idxs; auto.   } 
-    assert (Hsub':  sublist (b + 1) BINS (zip3 lens bins idxs)  
-                  = sublist (b + 1) BINS (zip3 lens' bins' idxs)).
-    { repeat rewrite sublist_zip3; try rep_omega.
-      - rewrite Hbins''. rewrite Hlens''.  reflexivity.
-      - unfold lens'; rewrite upd_Znth_Zlength; repeat rep_omega.
-      - unfold lens'; unfold bins'; rewrite upd_Znth_Zlength.
-        rewrite upd_Znth_Zlength; rep_omega. rep_omega.
-      - replace (Zlength bins') with BINS by auto. unfold idxs; auto.
-      - unfold idxs; auto.   } 
-    rewrite Hsub. rewrite Hsub'.
-    (* Here's a place where it would be nice if sep_apply could do rewriting *)
-    rewrite pull_right.
-    assert (Hq: q = (Znth b bins')). (* TODO clean this mess *)
-    { unfold bins'. rewrite upd_Znth_same.  
-      destruct q; auto with valid_pointer.
-      match goal with | HA: Zlength bins = _ |- _ => 
-                        auto 10  with valid_pointer; rewrite H0; assumption end. 
-    }
-    rewrite Hq.
-    (* Annoying rewrite, but can't use replace_SEP because that's for 
-       preconditions; would have to do use it back at the last forward. *)
-    assert (Hassoc:
-        iter_sepcon mmlist' (sublist 0 b (zip3 lens' bins' idxs)) *
-        mmlist (bin2sizeZ b) (Znth b lens') (Znth b bins') nullval * TT *
-        iter_sepcon mmlist' (sublist (b + 1) BINS (zip3 lens' bins' idxs))
-      = iter_sepcon mmlist' (sublist 0 b (zip3 lens' bins' idxs)) *
-        iter_sepcon mmlist' (sublist (b + 1) BINS (zip3 lens' bins' idxs)) *
-        mmlist (bin2sizeZ b) (Znth b lens') (Znth b bins') nullval * TT)
-           by (apply pred_ext; entailer!).
-    rewrite Hassoc; clear Hassoc. 
-    rewrite mm_inv_split'; try entailer!; auto.
-    subst lens'; rewrite upd_Znth_Zlength; rewrite H1; auto.
-    (* field_compatible t p *)
-    destruct H as [Hsiz [Hcosu Halign]].
-    apply malloc_compatible_field_compatible; try assumption.
-Qed.
 
 
 
-Lemma body_free_small:  semax_body Vprog Gprog f_free_small free_small_spec.
-Proof. 
-start_function. 
-destruct H as [[Hn Hn'] [Hs Hmc]].
-forward_call s. (*! b = size2bin(s) !*)
-{ subst; pose proof (bin2size_range(size2binZ n)); pose proof (claim2 n); rep_omega. }
-set (b:=(size2binZ n)). 
-assert (Hb: b = size2binZ s) by (subst; rewrite claim3; auto).
-rewrite <- Hb.
-assert (Hb': 0 <= b < BINS) 
-  by (change b with (size2binZ n); apply claim2; split; assumption).
-rewrite (mm_inv_split gv b Hb'). (* to expose bins[b] in mm_inv *)
-Intros bins lens idxs.
-forward. (*! void *q = bin[b] !*) 
-assert_PROP( (force_val (sem_cast_pointer p) = field_address (tptr tvoid) [] p) ). 
-{ entailer!. unfold field_address; normalize; if_tac; auto; contradiction. }
-forward. (*!  *((void ** )p) = q !*)
-gather_SEP 0 1 2 5.
-set (q:=(Znth b bins)).
-assert_PROP (p <> nullval) by entailer!.
-apply semax_pre with 
-    (PROP ( )
-     LOCAL (temp _q q; temp _b (Vint (Int.repr b)); 
-     temp _p p; temp _s (Vptrofs (Ptrofs.repr s)); gvars gv)
-     SEP ((EX q': val, 
-!!(malloc_compatible s p 
-   /\ p <> nullval) && 
-          data_at Tsh tuint (Vptrofs (Ptrofs.repr s)) (offset_val (- WORD) p) *
-          data_at Tsh (tptr tvoid) q' p *
-          memory_block Tsh (s - WORD) (offset_val WORD p) *
-          mmlist (bin2sizeZ b) (Znth b lens) q' nullval) ;
-     data_at Tsh (tarray (tptr tvoid) BINS) bins (gv _bin);
-     iter_sepcon mmlist' (sublist 0 b (zip3 lens bins idxs)) ;
-     iter_sepcon mmlist' (sublist (b + 1) BINS (zip3 lens bins idxs)) ;
-     TT)).
-{ Exists q. entailer!. }
-replace (bin2sizeZ b) with s by auto. 
-change (Znth b lens)
-  with (Nat.pred (Nat.succ (Znth b lens))).
-
-assert_PROP( isptr p ). 
-{ entailer!. unfold nullval in *.
-  match goal with | HA: p <> _ |- _ => simpl in HA end. (* not Archi.ptr64 *)
-  unfold is_pointer_or_null in *. simpl in *.
-  destruct p; try contradiction; simpl.  auto. 
-}
-assert (succ_pos: forall n:nat, Z.of_nat (Nat.succ n) > 0) 
-  by (intros; rewrite Nat2Z.inj_succ; rep_omega).
-rewrite <- (mmlist_unroll_nonempty s (Nat.succ (Znth b lens)) p nullval);
-  try assumption; try apply succ_pos. clear succ_pos.
-forward. (*! bin[b] = p !*)
-set (bins':=(upd_Znth b bins p)).
-set (lens':=(upd_Znth b lens (Nat.succ (Znth b lens)))).
-gather_SEP 1 2 3 0. 
-apply semax_pre with 
-    (PROP ( )
-     LOCAL (temp _q q; temp _b (Vint (Int.repr b)); 
-     temp _p p; temp _s (Vptrofs (Ptrofs.repr s)); gvars gv)
-     SEP (
-  EX bins1: list val, EX lens1: list nat, EX idxs1: list Z,
-  !! (Zlength bins1 = BINS /\ Zlength lens1 = BINS /\ Zlength idxs1 = BINS
-      /\ idxs1 = map Z.of_nat (seq 0 (Z.to_nat BINS))) &&
-    data_at Tsh (tarray (tptr tvoid) BINS) bins1 (gv _bin) * 
-    iter_sepcon mmlist' (sublist 0 b (zip3 lens1 bins1 idxs1)) *
-    mmlist (bin2sizeZ b) (Znth b lens1) (Znth b bins1) nullval *
-    iter_sepcon mmlist' (sublist (b + 1) BINS (zip3 lens1 bins1 idxs1)) *
-    TT )).
-{ Exists bins'. Exists lens'. Exists idxs.
-  assert_PROP(Zlength bins' = BINS /\ Zlength lens' = BINS).
-  { unfold bins'.  unfold lens'.  
-    rewrite (upd_Znth_Zlength b bins p); try omega.
-    match goal with |- context [upd_Znth b lens ?X] => set (foo:=X) end.
-    rewrite (upd_Znth_Zlength b lens foo); try omega. 
-    entailer!. 
-  }
-  replace (bin2sizeZ b) with s by auto. 
-  replace (bin2sizeZ b) with s by auto. 
-  replace (Znth b bins') with p 
-    by (unfold bins'; rewrite upd_Znth_same; auto; rewrite H; assumption). 
-  replace (Nat.succ (Znth b lens)) with (Znth b lens') 
-    by (unfold lens'; rewrite upd_Znth_same; try reflexivity; omega).
-  entailer!.
-  change (upd_Znth (size2binZ n) bins p) with bins'.  entailer!.
-  (* remains to show bins' and lens' are same as originals aside from n *)
-  set (idxs:=(map Z.of_nat (seq 0 (Z.to_nat BINS)))) in *.
-  repeat rewrite sublist_zip3; try rep_omega.
-  replace (sublist 0 (size2binZ n) lens') 
-     with (sublist 0 (size2binZ n) lens) by
-   (unfold lens'; rewrite sublist_upd_Znth_l; try reflexivity; try rep_omega).
-  replace (sublist (size2binZ n + 1) BINS lens') 
-     with (sublist (size2binZ n + 1) BINS lens) by 
-   (unfold lens'; rewrite sublist_upd_Znth_r; try reflexivity; try rep_omega).
-  replace (sublist 0 (size2binZ n) bins')
-     with (sublist 0 (size2binZ n) bins) by 
-   (unfold bins'; rewrite sublist_upd_Znth_l; try reflexivity; try rep_omega).
-  replace (sublist (size2binZ n + 1) BINS bins')
-     with (sublist (size2binZ n + 1) BINS bins) by 
-   (unfold bins'; rewrite sublist_upd_Znth_r; try reflexivity; try rep_omega).
-  entailer!.
-}
-rewrite <- (mm_inv_split gv b Hb'). 
-forward. (*! return !*) 
-Qed.
 
 
