memmgr/verif_bin2size2bin.v
@@ -1,0 +1,24 @@
+Require Import VST.floyd.proofauto.
+Require Import VST.floyd.library.
+Require Import VST.msl.iter_sepcon.
+Require Import malloc.
+Require Import verif_memmgr.
+
+Lemma body_bin2size: semax_body Vprog Gprog f_bin2size bin2size_spec.
+Proof. start_function. forward. 
+Qed.
+
+Lemma body_size2bin: semax_body Vprog Gprog f_size2bin size2bin_spec.
+Proof. start_function. 
+  forward_call (BINS-1). rep_omega. 
+  forward_if.
+  - (* then *) 
+    forward. entailer!. f_equal. f_equal. unfold size2binZ; simpl. 
+    bdestruct (bin2sizeZ (BINS - 1) <? s); try omega.
+  - (* else *)
+    forward.  entailer!. f_equal. unfold size2binZ. 
+    bdestruct (bin2sizeZ (BINS - 1) <? s); try omega.
+    unfold Int.divu. do 2 rewrite Int.unsigned_repr by rep_omega. 
+    f_equal. normalize.  f_equal. rep_omega.
+Qed.
+
