memmgr/verif_free_small.v
@@ -1,0 +1,110 @@
+Require Import VST.floyd.proofauto.
+Require Import VST.floyd.library.
+Require Import VST.msl.iter_sepcon.
+Require Import malloc.
+Require Import verif_memmgr.
+
+Lemma body_free_small:  semax_body Vprog Gprog f_free_small free_small_spec.
+Proof. 
+start_function. 
+destruct H as [[Hn Hn'] [Hs Hmc]].
+forward_call s. (*! b = size2bin(s) !*)
+{ subst; pose proof (bin2size_range(size2binZ n)); pose proof (claim2 n); rep_omega. }
+set (b:=(size2binZ n)). 
+assert (Hb: b = size2binZ s) by (subst; rewrite claim3; auto).
+rewrite <- Hb.
+assert (Hb': 0 <= b < BINS) 
+  by (change b with (size2binZ n); apply claim2; split; assumption).
+rewrite (mem_mgr_split gv b Hb'). (* to expose bins[b] in mem_mgr *)
+Intros bins lens idxs.
+forward. (*! void *q = bin[b] !*) 
+assert_PROP( (force_val (sem_cast_pointer p) = field_address (tptr tvoid) [] p) ). 
+{ entailer!. unfold field_address; normalize; if_tac; auto; contradiction. }
+forward. (*!  *((void ** )p) = q !*)
+gather_SEP 0 1 2 5.
+set (q:=(Znth b bins)).
+assert_PROP (p <> nullval) by entailer!.
+apply semax_pre with 
+    (PROP ( )
+     LOCAL (temp _q q; temp _b (Vint (Int.repr b)); 
+     temp _p p; temp _s (Vptrofs (Ptrofs.repr s)); gvars gv)
+     SEP ((EX q': val, 
+!!(malloc_compatible s p 
+   /\ p <> nullval) && 
+          data_at Tsh tuint (Vptrofs (Ptrofs.repr s)) (offset_val (- WORD) p) *
+          data_at Tsh (tptr tvoid) q' p *
+          memory_block Tsh (s - WORD) (offset_val WORD p) *
+          mmlist (bin2sizeZ b) (Znth b lens) q' nullval) ;
+     data_at Tsh (tarray (tptr tvoid) BINS) bins (gv _bin);
+     iter_sepcon mmlist' (sublist 0 b (zip3 lens bins idxs)) ;
+     iter_sepcon mmlist' (sublist (b + 1) BINS (zip3 lens bins idxs)) ;
+     TT)).
+{ Exists q. entailer!. }
+replace (bin2sizeZ b) with s by auto. 
+change (Znth b lens)
+  with (Nat.pred (Nat.succ (Znth b lens))).
+
+assert_PROP( isptr p ). 
+{ entailer!. unfold nullval in *.
+  match goal with | HA: p <> _ |- _ => simpl in HA end. (* not Archi.ptr64 *)
+  unfold is_pointer_or_null in *. simpl in *.
+  destruct p; try contradiction; simpl.  auto. 
+}
+assert (succ_pos: forall n:nat, Z.of_nat (Nat.succ n) > 0) 
+  by (intros; rewrite Nat2Z.inj_succ; rep_omega).
+rewrite <- (mmlist_unroll_nonempty s (Nat.succ (Znth b lens)) p nullval);
+  try assumption; try apply succ_pos. clear succ_pos.
+forward. (*! bin[b] = p !*)
+set (bins':=(upd_Znth b bins p)).
+set (lens':=(upd_Znth b lens (Nat.succ (Znth b lens)))).
+gather_SEP 1 2 3 0. 
+apply semax_pre with 
+    (PROP ( )
+     LOCAL (temp _q q; temp _b (Vint (Int.repr b)); 
+     temp _p p; temp _s (Vptrofs (Ptrofs.repr s)); gvars gv)
+     SEP (
+  EX bins1: list val, EX lens1: list nat, EX idxs1: list Z,
+  !! (Zlength bins1 = BINS /\ Zlength lens1 = BINS /\ Zlength idxs1 = BINS
+      /\ idxs1 = map Z.of_nat (seq 0 (Z.to_nat BINS))) &&
+    data_at Tsh (tarray (tptr tvoid) BINS) bins1 (gv _bin) * 
+    iter_sepcon mmlist' (sublist 0 b (zip3 lens1 bins1 idxs1)) *
+    mmlist (bin2sizeZ b) (Znth b lens1) (Znth b bins1) nullval *
+    iter_sepcon mmlist' (sublist (b + 1) BINS (zip3 lens1 bins1 idxs1)) *
+    TT )).
+{ Exists bins'. Exists lens'. Exists idxs.
+  assert_PROP(Zlength bins' = BINS /\ Zlength lens' = BINS).
+  { unfold bins'.  unfold lens'.  
+    rewrite (upd_Znth_Zlength b bins p); try omega.
+    match goal with |- context [upd_Znth b lens ?X] => set (foo:=X) end.
+    rewrite (upd_Znth_Zlength b lens foo); try omega. 
+    entailer!. 
+  }
+  replace (bin2sizeZ b) with s by auto. 
+  replace (bin2sizeZ b) with s by auto. 
+  replace (Znth b bins') with p 
+    by (unfold bins'; rewrite upd_Znth_same; auto; rewrite H; assumption). 
+  replace (Nat.succ (Znth b lens)) with (Znth b lens') 
+    by (unfold lens'; rewrite upd_Znth_same; try reflexivity; omega).
+  entailer!.
+  change (upd_Znth (size2binZ n) bins p) with bins'.  entailer!.
+  (* remains to show bins' and lens' are same as originals aside from n *)
+  set (idxs:=(map Z.of_nat (seq 0 (Z.to_nat BINS)))) in *.
+  repeat rewrite sublist_zip3; try rep_omega.
+  replace (sublist 0 (size2binZ n) lens') 
+     with (sublist 0 (size2binZ n) lens) by
+   (unfold lens'; rewrite sublist_upd_Znth_l; try reflexivity; try rep_omega).
+  replace (sublist (size2binZ n + 1) BINS lens') 
+     with (sublist (size2binZ n + 1) BINS lens) by 
+   (unfold lens'; rewrite sublist_upd_Znth_r; try reflexivity; try rep_omega).
+  replace (sublist 0 (size2binZ n) bins')
+     with (sublist 0 (size2binZ n) bins) by 
+   (unfold bins'; rewrite sublist_upd_Znth_l; try reflexivity; try rep_omega).
+  replace (sublist (size2binZ n + 1) BINS bins')
+     with (sublist (size2binZ n + 1) BINS bins) by 
+   (unfold bins'; rewrite sublist_upd_Znth_r; try reflexivity; try rep_omega).
+  entailer!.
+}
+rewrite <- (mem_mgr_split gv b Hb'). 
+forward. (*! return !*) 
+Qed.
+
