memmgr/verif_malloc_free.v
@@ -1,0 +1,104 @@
+Require Import VST.floyd.proofauto.
+Require Import VST.floyd.library.
+Require Import VST.msl.iter_sepcon.
+Require Import malloc.
+Require Import verif_memmgr.
+
+Lemma body_malloc:  semax_body Vprog Gprog f_malloc malloc_spec.
+Proof. 
+start_function. 
+forward_call (BINS-1). (*! t'3 = bin2size(BINS-1) !*)
+rep_omega. 
+forward_if. (*! if nbytes > t'3 !*)
+- (* case nbytes > bin2size(BINS-1) *)
+  forward_call (t, gv).  (*! t'1 = malloc_large(nbytes) !*)
+  { (* precond *) 
+    destruct H. split3; try assumption. split; try rep_omega. 
+    assert (0 <= sizeof t) as H' by omega.
+    pose proof (unsigned_repr_le (sizeof t) H').
+    eapply Z.lt_le_trans. 
+    match goal with | HA: bin2sizeZ (BINS-1) < _ |- _ => apply HA end. 
+    assumption.
+  } 
+  Intros p.
+  forward. (*! return t'1 !*) 
+  if_tac.
+  + (* case p = null *) Exists nullval. entailer!.
+    if_tac; try contradiction. entailer!. 
+  + Exists p. if_tac. contradiction. 
+    entailer!.  
+- (* case nbytes <= bin2size(BINS-1) *)
+  forward_call(t,gv).  (*! t'2 = malloc_small(nbytes) !*)
+  { (* precond *)
+    destruct H. split3; try assumption. 
+    split; try rep_omega. 
+    clear H0 H1.
+    match goal with | HA: bin2sizeZ (BINS-1) >= _ |- _ => apply Z.ge_le in HA end.
+    rewrite max_unsigned_32 in *.
+    rewrite Int.unsigned_repr in *; try assumption. 
+    split; try omega. 
+    apply Z.lt_le_incl; assumption.
+    assert (0 <= WA+WORD) as HA by rep_omega.
+    eapply Z.le_le_sub_lt; try apply HA.
+    replace (sizeof t - 0) with (sizeof t).
+    assumption.
+    rewrite Z.sub_0_r; reflexivity.
+  }
+  Intros p.
+  forward. (*! result = t'2 !*)
+  Exists p. 
+  entailer!.
+Qed.
+
+Lemma body_free:  semax_body Vprog Gprog f_free free_spec.
+Proof. 
+start_function. 
+set (n:=sizeof t). (* try to avoid entailer or rep_omega issues *)
+forward_if (PROP()LOCAL()SEP(mem_mgr gv)). (*! if (p != NULL) !*)
+- (* typecheck *) if_tac. entailer!.
+  assert_PROP( 0 < n ) by (unfold malloc_token; unfold malloc_tok; entailer).
+  sep_apply (data_at__memory_block Tsh t p). 
+  entailer!.
+- (* case p!=NULL *)
+  apply semax_pre with 
+   (PROP ( )
+     LOCAL (temp _p p; gvars gv)
+     SEP (mem_mgr gv;  malloc_token Tsh t p * data_at_ Tsh t p)).
+  { if_tac; entailer!. }
+  assert_PROP ( 0 <= n <= Ptrofs.max_unsigned - WORD ) by entailer!. 
+  sep_apply (from_malloc_token_and_block t n p); auto.
+  Intros s.
+  assert_PROP( 
+     (force_val
+     (sem_add_ptr_int tuint Signed (force_val (sem_cast_pointer p))
+        (eval_unop Oneg tint (Vint (Int.repr 1)))) 
+    = field_address tuint [] (offset_val (- WORD) p))).
+  { entailer!. simpl. unfold field_address. if_tac. normalize. contradiction. }
+  forward. (*! t'2 = p[-1] !*)
+  forward. (*! s = t'2 !*) 
+  forward_call(BINS - 1). (*! t'1 = bin2size(BINS - 1) !*)
+  { (* precond *) rep_omega. } 
+  deadvars!.
+  forward_if (PROP () LOCAL () SEP (mem_mgr gv)). (*! if s <= t'1 !*)
+  -- (* case s <= bin2sizeZ(BINS-1) *)
+    forward_call(p,s,n,gv). (*! free_small(p,s) !*) 
+    { (* preconds *) split3; try omega; try assumption. }
+    entailer!. if_tac. entailer. omega.
+  -- (* case s > bin2sizeZ(BINS-1) *)
+    if_tac; try omega.
+    (*! munmap( p-(WASTE+WORD), s+WASTE+WORD ) !*)
+    forward_call( (offset_val (-(WA+WORD)) p), (s+WA+WORD) ).
+    + entailer!. destruct p; try contradiction; simpl. normalize.
+      rewrite Ptrofs.sub_add_opp. reflexivity.
+    + (* munmap pre *)
+      entailer!. 
+      sep_apply (free_large_chunk s p); try rep_omega.
+      entailer!.
+    + rep_omega.
+    + entailer!.
+- (* case p == NULL *) 
+  forward. (*! skip !*)
+  entailer!.
+- (* after if *)
+  forward. (*! return !*)
+Qed.
