memmgr/verif_malloc_large.v
@@ -1,0 +1,95 @@
+Require Import VST.floyd.proofauto.
+Require Import VST.floyd.library.
+Require Import VST.msl.iter_sepcon.
+Require Import malloc.
+Require Import verif_memmgr.
+
+Lemma body_malloc_large: semax_body Vprog Gprog f_malloc_large malloc_large_spec.
+Proof.
+start_function. 
+set (n:= sizeof t).
+forward_call (n+WA+WORD). (*! t'1 = mmap0(nbytes+WASTE+WORD ...) !*)
+{ rep_omega. }
+Intros p.
+(* NOTE could split cases here; then two symbolic executions but simpler ones *)
+forward_if. (*! if (p==NULL) !*)
+- (* typecheck guard *) 
+  if_tac; entailer!.
+- (* case p == NULL *) 
+  forward. (*! return NULL  !*)
+  Exists (Vint (Int.repr 0)).
+  if_tac; entailer!. (* cases in post of mmap *)
+- (* case p <> NULL *) 
+  if_tac. (* cases in post of mmap *)
+  + (* impossible case *)
+    elimtype False. destruct p; try contradiction; simpl in *.
+  + assert_PROP (
+        (force_val
+           (sem_add_ptr_int tuint Signed
+                            (force_val
+                               (sem_cast_pointer
+                                  (force_val
+                                     (sem_add_ptr_int tschar Unsigned p
+                                                      (Vint
+                                                         (Int.sub
+                                                            (Int.mul (Ptrofs.to_int (Ptrofs.repr 4)) (Int.repr 2))
+                                                            (Ptrofs.to_int (Ptrofs.repr 4))))))))
+                            (Vint (Int.repr 0))) = field_address tuint [] (offset_val WA p)) ).
+    (* painful pointer reasoning to enable forward (p+WASTE)[0] = nbytes *)
+    { entailer!. 
+      destruct p; try contradiction; simpl.
+      normalize.
+      unfold field_address.
+      rewrite if_true.
+      { simpl.  normalize. }
+      hnf. (* drill down *) 
+      repeat split; auto.
+      - (* size compat *)
+        red. 
+        match goal with | H:size_compatible' _ _ |- _ => red in H end.
+        unfold Ptrofs.add.
+        rewrite (Ptrofs.unsigned_repr WA) by rep_omega.
+        rewrite Ptrofs.unsigned_repr by rep_omega.
+        simpl sizeof. rep_omega.
+      - (* align compat *)
+        red.
+        eapply align_compatible_rec_by_value; try reflexivity.
+        simpl in *. unfold natural_alignment in *. unfold Z.divide in *.
+        match goal with | HA: (exists z:Z, _) /\ _ |- _ => destruct HA as [Hz Hlim] end. 
+        inv Hz.
+        rewrite <- (Ptrofs.repr_unsigned i). 
+        match goal with | HA: Ptrofs.unsigned _ = _ |- _ => rewrite HA end. 
+        exists (2*x+1). change WA with 4.
+        rewrite ptrofs_add_repr. rewrite Ptrofs.unsigned_repr.
+        omega. rep_omega.
+    }
+    rewrite malloc_large_chunk; try rep_omega; try assumption.
+    Intros. (* flatten sep *)
+    forward. (*! (p+WASTE)[0] = nbytes;  !*)
+    forward. (*! return (p+WASTE+WORD);  !*)
+    (* postcond *)
+    Exists (offset_val (WA+WORD) p).
+    entailer!.  
+    if_tac. 
+    { elimtype False. destruct p; try contradiction; simpl in *. 
+      match goal with | HA: Vptr _ _  = nullval |- _ => inv HA end. }
+    entailer!.
+    unfold malloc_token.
+    Exists n.
+    unfold malloc_tok.
+    if_tac. rep_omega. entailer!. 
+    { apply malloc_compatible_offset; try rep_omega; try apply WORD_ALIGN_aligned.
+      replace (n+(WA+WORD)) with (n + WA + WORD) by omega. assumption. }
+    cancel.
+    (* data_at_ from memory_block *)
+    replace (n - sizeof t) with 0 by omega.
+    rewrite memory_block_zero.  entailer!.
+    subst n.
+    rewrite memory_block_data_at_. entailer!.
+    destruct H as [Hsz [Hcosu Halign]]; auto.
+    apply malloc_compatible_field_compatible; try auto.
+    apply malloc_compatible_offset; try rep_omega.
+    replace (sizeof t + (WA + WORD)) with (sizeof t + WA + WORD) by omega; assumption.
+    apply WORD_ALIGN_aligned.
+Qed.
+
