memmgr/verif_malloc_small.v
@@ -1,0 +1,203 @@
+Require Import VST.floyd.proofauto.
+Require Import VST.floyd.library.
+Require Import VST.msl.iter_sepcon.
+Require Import malloc.
+Require Import verif_memmgr.
+
+
+Lemma body_malloc_small:  semax_body Vprog Gprog f_malloc_small malloc_small_spec.
+Proof. 
+start_function. 
+set (n := sizeof t).
+rewrite <- seq_assoc.  
+forward_call n. (*! t'1 = size2bin(nbytes) !*)
+{ assert (bin2sizeZ(BINS-1) <= Ptrofs.max_unsigned) by rep_omega. rep_omega. }
+forward. (*! b = t'1 !*)
+set (b:=size2binZ n).
+assert (Hb: 0 <= b < BINS) by (apply (claim2 n); omega). 
+rewrite (mem_mgr_split gv b) by apply Hb.
+Intros bins lens idxs.
+freeze [1; 3] Otherlists.
+deadvars!.
+forward. (*! p = bin[b] !*)
+forward_if(
+    EX p:val, EX len:Z,
+     PROP(p <> nullval)
+     LOCAL(temp _p p; temp _b (Vint (Int.repr b)); gvars gv)
+     SEP(FRZL Otherlists; TT; 
+         data_at Tsh (tarray (tptr tvoid) BINS) (upd_Znth b bins p) (gv _bin);
+         mmlist (bin2sizeZ b) (Z.to_nat len) p nullval)). 
+
+  + (* typecheck guard *)
+    destruct (Znth b lens). 
+    match goal with | HA: Znth b bins = nullval <-> _ |- _ => set (Hbn:=HA) end. 
+    (*Set Printing Implicit. -- to see the need for following step. *)
+    change Inhabitant_val with Vundef in Hbn.
+    ++ assert (Znth b bins = nullval) by apply (proj2 Hbn (eq_refl _)).
+       change (@Znth val Vundef) with (@Znth val Inhabitant_val).
+       replace (Znth b bins) with nullval by assumption.
+       auto with valid_pointer.
+    ++ match goal with | HA: Znth b bins = nullval <-> _ |- _ => destruct HA end.
+       assert (Znth b bins <> nullval) by
+           (assert (S n0 <> 0%nat) by congruence; auto).
+       change (Vint Int.zero) with nullval.
+       auto with valid_pointer.
+       apply denote_tc_test_eq_split; auto with valid_pointer.
+       sep_apply (mmlist_ne_valid_pointer (bin2sizeZ b) (S n0) (Znth b bins) nullval).
+       omega. change Inhabitant_val with Vundef; entailer!.
+  + (* case p==NULL *) 
+    change Inhabitant_val with Vundef in *.
+    replace (Znth b bins) with nullval by assumption.
+    assert_PROP(Znth b lens = 0%nat) as Hlen0.
+    { entailer!.
+      match goal with | HA: nullval = nullval <-> _ |- _ => (apply HA; reflexivity) end.
+    } 
+    rewrite Hlen0.
+    rewrite mmlist_empty.
+    forward_call b. (*! p = fill_bin(b) !*) 
+    Intro r_with_l; destruct r_with_l as [root len]; simpl.
+    forward_if. (*! if p==NULL !*)
+    { apply denote_tc_test_eq_split; auto with valid_pointer.
+      if_tac. entailer!.
+      sep_apply (mmlist_ne_valid_pointer (bin2sizeZ b) (Z.to_nat len) root nullval).
+      change (Z.to_nat len > 0)%nat with (0 < Z.to_nat len)%nat.
+      change 0%nat with (Z.to_nat 0). apply Z2Nat.inj_lt; rep_omega.
+      entailer!.
+    }
+    ++ (* case p==NULL after fill_bin() *) 
+      forward.
+      Exists nullval. entailer!. 
+      thaw Otherlists.
+      set (idxs:= (map Z.of_nat (seq 0 (Z.to_nat BINS)))).
+      replace (data_at Tsh (tarray (tptr tvoid) BINS) bins (gv _bin))
+         with (data_at Tsh (tarray (tptr tvoid) BINS) bins (gv _bin) * emp) 
+         by normalize.
+      rewrite <- (mmlist_empty (bin2sizeZ b)) at 2.
+      rewrite <- Hlen0 at 1.
+      unfold mem_mgr. Exists bins. Exists lens. Exists idxs.
+      entailer!. 
+      match goal with | HA: (Znth b bins = _) |- _ => rewrite <- HA at 1 end.
+      rewrite (mem_mgr_split' b); auto.  
+      pose proof (bin2size_range b); rep_omega.
+    ++ (* case p<>NULL *)
+      if_tac. contradiction.
+      gather_SEP 0 1. 
+      Intros.
+      forward. (*! bin[b] = p !*)
+      Exists root. Exists len.  
+      entailer. cancel. 
+    ++ pose proof (bin2size_range b); rep_omega.
+  + (* else branch p!=NULL *)
+    forward. (*! skip !*)
+    Exists (Znth b bins).  
+    Exists (Z.of_nat (nth (Z.to_nat b) lens 0%nat)). (* annoying conversion *)
+    rewrite Nat2Z.id.  
+    match goal with | HA: Zlength bins = _ |- _ => 
+                      rewrite upd_Znth_same_val by (rewrite HA; assumption) end. 
+    entailer!.
+    match goal with | HA: Zlength lens = _ |- _ => 
+                      rewrite <- nth_Znth by (rewrite HA; assumption) end.  
+    entailer.
+  + (* after if: unroll and pop mmlist *)
+    Intros p len.
+    set (s:=bin2sizeZ b).  
+    assert_PROP (len > 0).
+    { entailer. sep_apply (mmlist_ne_len s len p nullval); auto.
+      rewrite prop_sepcon. entailer!.  }
+    assert_PROP (isptr p).
+    { entailer!. unfold nullval in *.
+      match goal with | HA: p <> _ |- _ => simpl in HA end. (* not Archi.ptr64 *)
+      unfold is_pointer_or_null in *. simpl in *.
+      destruct p; try contradiction; simpl.
+      subst. contradiction. auto. }
+    rewrite (mmlist_unroll_nonempty s (Z.to_nat len) p);
+       try (rewrite Z2Nat.id; rep_omega); try assumption.
+    Intros q.
+    assert_PROP(force_val (sem_cast_pointer p) = field_address (tptr tvoid) [] p).
+    { entailer!. unfold field_address. if_tac. normalize. contradiction. }
+    forward. (*! q = *p !*)
+    forward. (*! bin[b]=q !*)
+    (* prepare token+chunk to return *)
+    deadvars!.
+    thaw Otherlists.  gather_SEP 4 5 6.
+    replace_SEP 0 (malloc_token Tsh t p * memory_block Tsh n p). 
+    go_lower.  change (-4) with (-WORD). (* ugh *)
+    apply (to_malloc_token_and_block n p q s); try assumption. 
+    destruct H as [? [? ?]].
+    unfold n; auto.
+    unfold s; unfold b; reflexivity. 
+    (* refold invariant *)
+    rewrite upd_Znth_twice by (rewrite H0; apply Hb).
+    gather_SEP 4 1 5.
+    set (lens':=(upd_Znth b lens (Nat.pred (Z.to_nat len)))).
+    set (bins':=(upd_Znth b bins (force_val (sem_cast_pointer q)))).
+    assert (Hlens: Nat.pred (Z.to_nat len) = (Znth b lens')).
+    { unfold lens'. rewrite upd_Znth_same. reflexivity. 
+      match goal with | HA: Zlength lens = _ |- _ => rewrite HA end. 
+      assumption. }
+    rewrite Hlens; clear Hlens.
+    change s with (bin2sizeZ b).
+    forward. (*! return p !*)
+    Exists p. entailer!. if_tac. contradiction. cancel.
+    unfold mem_mgr. Exists bins'. Exists lens'. 
+    set (idxs:= (map Z.of_nat (seq 0 (Z.to_nat BINS)))).
+    Exists idxs. cancel.
+    subst n.
+    rewrite memory_block_data_at_.
+    entailer!.
+    match goal with | HA: Zlength lens = _ |- _ => 
+                      subst lens'; rewrite upd_Znth_Zlength; rewrite HA; auto end.
+    (* fold mem_mgr *)
+    assert (Hbins': sublist 0 b bins' = sublist 0 b bins) by
+      (unfold bins'; rewrite sublist_upd_Znth_l; try reflexivity; try rep_omega).
+    assert (Hlens': sublist 0 b lens' = sublist 0 b lens) by 
+      (unfold lens'; rewrite sublist_upd_Znth_l; try reflexivity; try rep_omega).
+    assert (Hbins'': sublist (b+1) BINS bins' = sublist (b+1) BINS bins) by
+      (unfold bins'; rewrite sublist_upd_Znth_r; try reflexivity; try rep_omega).
+    assert (Hlens'': sublist (b+1) BINS lens' = sublist (b+1) BINS lens) by
+      (unfold lens'; rewrite sublist_upd_Znth_r; try reflexivity; try rep_omega).
+    assert (Hsub:  sublist 0 b (zip3 lens bins idxs)
+                 = sublist 0 b (zip3 lens' bins' idxs)).
+    { repeat rewrite sublist_zip3; try rep_omega.
+      - rewrite Hbins'. rewrite Hlens'.  reflexivity.
+      - unfold lens'; rewrite upd_Znth_Zlength; repeat rep_omega.
+      - unfold lens'; unfold bins'; rewrite upd_Znth_Zlength.
+        rewrite upd_Znth_Zlength; rep_omega. rep_omega.
+      - replace (Zlength bins') with BINS by auto. unfold idxs; auto.
+      - unfold idxs; auto.   } 
+    assert (Hsub':  sublist (b + 1) BINS (zip3 lens bins idxs)  
+                  = sublist (b + 1) BINS (zip3 lens' bins' idxs)).
+    { repeat rewrite sublist_zip3; try rep_omega.
+      - rewrite Hbins''. rewrite Hlens''.  reflexivity.
+      - unfold lens'; rewrite upd_Znth_Zlength; repeat rep_omega.
+      - unfold lens'; unfold bins'; rewrite upd_Znth_Zlength.
+        rewrite upd_Znth_Zlength; rep_omega. rep_omega.
+      - replace (Zlength bins') with BINS by auto. unfold idxs; auto.
+      - unfold idxs; auto.   } 
+    rewrite Hsub. rewrite Hsub'.
+    (* Here's a place where it would be nice if sep_apply could do rewriting *)
+    rewrite pull_right.
+    assert (Hq: q = (Znth b bins')). (* TODO clean this mess *)
+    { unfold bins'. rewrite upd_Znth_same.  
+      destruct q; auto with valid_pointer.
+      match goal with | HA: Zlength bins = _ |- _ => 
+                        auto 10  with valid_pointer; rewrite H0; assumption end. 
+    }
+    rewrite Hq.
+    (* Annoying rewrite, but can't use replace_SEP because that's for 
+       preconditions; would have to do use it back at the last forward. *)
+    assert (Hassoc:
+        iter_sepcon mmlist' (sublist 0 b (zip3 lens' bins' idxs)) *
+        mmlist (bin2sizeZ b) (Znth b lens') (Znth b bins') nullval * TT *
+        iter_sepcon mmlist' (sublist (b + 1) BINS (zip3 lens' bins' idxs))
+      = iter_sepcon mmlist' (sublist 0 b (zip3 lens' bins' idxs)) *
+        iter_sepcon mmlist' (sublist (b + 1) BINS (zip3 lens' bins' idxs)) *
+        mmlist (bin2sizeZ b) (Znth b lens') (Znth b bins') nullval * TT)
+           by (apply pred_ext; entailer!).
+    rewrite Hassoc; clear Hassoc. 
+    rewrite mem_mgr_split'; try entailer!; auto.
+    subst lens'; rewrite upd_Znth_Zlength; rewrite H1; auto.
+    (* field_compatible t p *)
+    destruct H as [Hsiz [Hcosu Halign]].
+    apply malloc_compatible_field_compatible; try assumption.
+Qed.
